Charge!/src/Open/Stack.v
@@ -1,4 +1,4 @@
-Require Import Rel.
+Require Import Rel String.
 Require Import FunctionalExtensionality.
 
 Set Implicit Arguments.
@@ -11,33 +11,32 @@ Class ValNull := {
 }.
 
 Section Defs.
-  Context {A : Type} {H: DecidableEq A}.
   Context {B : ValNull}.
 
-  Definition stack := A -> val.
+  Definition stack := string -> val.
 
   Definition stack_empty : stack := fun x => null.
 
   Definition stack_add x v s : stack :=
-    fun x' => if dec_eq x' x then v else s x'.
+    fun x' => if string_dec x' x then v else s x'.
 
-  Lemma stack_lookup_add (s : stack) (x : A) (v : val) :
+  Lemma stack_lookup_add (s : stack) (x : string) (v : val) :
       ((stack_add x v s) : stack) x = v.
   Proof.
-    unfold stack_add. destruct (dec_eq x x); congruence.
+    unfold stack_add. destruct (string_dec x x); congruence.
   Qed.
 
-  Lemma stack_lookup_add2 (x y : A) (v : val) (s : stack) (Hneq: x <> y) :
+  Lemma stack_lookup_add2 (x y : string) (v : val) (s : stack) (Hneq: x <> y) :
     (stack_add x v s) y = s y.
   Proof.
-    unfold stack_add. destruct (dec_eq y x); congruence.
+    unfold stack_add. destruct (string_dec y x); congruence.
   Qed.
 
   Lemma stack_add_same (s: stack) x:
     stack_add x (s x) s = s.
   Proof.
     apply functional_extensionality.
-    intro x'. unfold stack_add. destruct (dec_eq x' x); [rewrite e|];
+    intro x'. unfold stack_add. destruct (string_dec x' x); [rewrite Heq|];
     reflexivity.
   Qed.
 
@@ -45,15 +44,15 @@ Section Defs.
     stack_add x v (stack_add x v' s) = stack_add x v s.
   Proof.
     apply functional_extensionality.
-    intro x'. unfold stack_add. destruct (dec_eq x' x); reflexivity.
+    intro x'. unfold stack_add. destruct (string_dec x' x); reflexivity.
   Qed.
   
-  Lemma stack_add_val_eq (s : stack) (x : A) v1 v2 (Hs : stack_add x v1 s = stack_add x v2 s) :
+  Lemma stack_add_val_eq (s : stack) (x : string) v1 v2 (Hs : stack_add x v1 s = stack_add x v2 s) :
   	v1 = v2.
   Proof.
     assert (stack_add x v1 s x = stack_add x v2 s x).
     rewrite Hs. reflexivity.
-    do 2 rewrite stack_lookup_add in H0. apply H0.
+    do 2 rewrite stack_lookup_add in H. apply H.
   Qed.
   
 End Defs.
