Charge!/src/Open/Subst.v
@@ -1,4 +1,4 @@
-Require Import Stack Open Rel.
+Require Import Stack Open Rel String.
 Require Import List FunctionalExtensionality.
 
 Set Implicit Arguments.
@@ -14,37 +14,36 @@ Fixpoint zip {A} {B} (lst1 : list A) (lst2 : list B) : list (A * B) :=
   end.
 
 Section Subst.
-  Context {A : Type} `{HEq: DecidableEq A}.
   Context {R : ValNull}.
 
-  Definition subst := A -> @open A R val.
+  Polymorphic Definition subst := string -> @open R val.
 
-  Definition stack_subst (s: stack A) (sub: subst) : stack A :=
+  Definition stack_subst (s: stack) (sub: subst) : stack :=
     fun x => sub x s.
 
   Definition apply_subst {B}
-          (e : @open A R B) (sub : subst) : @open A R B :=
+          (e : @open R B) (sub : subst) : @open R B :=
     fun s => e (stack_subst s sub).
 
-  Definition substlist := list (A * @expr A R).
+  Definition substlist := list (string * @expr R).
 
   (* The identity substitution *)
   Definition subst0 : subst := fun x => x/V.
 
   (* Substitution of one variable *)
   Definition subst1 e x : subst :=
-    fun x' => if dec_eq x' x then e else x'/V.
+    fun x' => if string_dec x' x then e else x'/V.
 
   (* Truncating substitution of one variable *)
   Definition subst1_trunc e x : subst :=
-    fun x' => if dec_eq x' x then e else empty_open.
+    fun x' => if string_dec x' x then e else empty_open.
 
   (* Simultaneous substitution of a finite list of variables *)
   Fixpoint substl_aux (subs: substlist) : subst :=
     match subs with
       | nil => subst0
       | (x,e) :: subs' => fun x' => 
-        if dec_eq x' x then e else substl_aux subs' x'
+        if string_dec x' x then e else substl_aux subs' x'
     end.
 
 (* Truncating simultaneous substitution of a finite list of variables *)
@@ -52,7 +51,7 @@ Section Subst.
     match subs with
       | nil => fun _ => empty_open
       | (x,e) :: subs' => fun x' => 
-        if dec_eq x' x then e else substl_trunc_aux subs' x'
+        if string_dec x' x then e else substl_trunc_aux subs' x'
     end.
 
   Definition substl es v := substl_aux es v.
@@ -78,22 +77,22 @@ Section Properties.
   Context {A : Type} `{Heq: DecidableEq A}.
   Context {R : ValNull}.
 
-  Lemma open_subst_stack {B} (m: @open A R B) (sub : subst) (s : @stack A R) :
+  Lemma open_subst_stack {B} (m: @open R B) (sub : subst) (s : @stack R) :
     (apply_subst m sub) s = m (stack_subst s sub).
   Proof. reflexivity. Qed.
 
-  Lemma subst0_id B (g: @open A R B) : (apply_subst g (@subst0 A R)) = g.
+  Lemma subst0_id B (g: @open R B) : (apply_subst g (@subst0 R)) = g.
   Proof.
     apply functional_extensionality.
     intros s; simpl; reflexivity.
   Qed.
 
-  Lemma subst1_stack (s: @stack A R) e x :
+  Lemma subst1_stack (s: @stack R) e x :
     stack_subst s (subst1 e x) = stack_add x (e s) s.
   Proof.
     apply functional_extensionality; intro x'; simpl.
     unfold stack_subst, subst1, stack_add. 
-    destruct (dec_eq x' x); reflexivity.
+    destruct (string_dec x' x); reflexivity.
   Qed.
 
   Lemma substl_subst1 x e :
@@ -109,7 +108,7 @@ Section Properties.
   Qed.
 
   Local Open Scope open_scope.
-  Lemma subst1_stack_add {B} (p : open B) (e : expr) (x : A) (v : val) (s : @stack A R) : 
+  Lemma subst1_stack_add {B} (p : open B) (e : expr) (x : string) (v : val) (s : @stack R) : 
     p[{e//x}] (stack_add x v s) = p[{e[{`v//x}]//x}] s.
   Proof.
     unfold apply_subst, subst1; simpl.
@@ -117,12 +116,12 @@ Section Properties.
     unfold stack_subst.
     apply functional_extensionality.
     intros y.
-    remember (dec_eq y x) as d.
+    remember (string_dec y x) as d.
     destruct d; simpl.
     apply f_equal.
     apply functional_extensionality.
     intros z; simpl.
-    remember (dec_eq z x) as d'.
+    remember (string_dec z x) as d'.
     destruct d'; subst.
     rewrite stack_lookup_add. reflexivity.
     rewrite stack_lookup_add2. reflexivity.
@@ -132,18 +131,18 @@ Section Properties.
     intuition.
   Qed.
       
-  Lemma stack_add_var (x : A) (s : @stack A R) (v : val) : (x/V) (stack_add x v s) = v.
+  Lemma stack_add_var (x : string) (s : @stack R) (v : val) : (x/V) (stack_add x v s) = v.
   Proof.
     unfold var_expr. rewrite stack_lookup_add. reflexivity.
   Qed.
   
-  Lemma subst1_val (v : val) (e : open val) (x : A) :
+  Lemma subst1_val (v : val) (e : open val) (x : string) :
     `v[{e//x}] = `v.
   Proof.
     reflexivity.
   Qed.
 
-  Lemma subst_identity {B} (x : A) (s : @stack A R) (p : open B) :
+  Lemma subst_identity {B} (x : string) (s : @stack R) (p : open B) :
     p[{`(s x)//x}] s = p s.
   Proof.
     unfold subst1, apply_subst.
@@ -151,28 +150,28 @@ Section Properties.
     unfold stack_subst; simpl.
     apply functional_extensionality.
     intros y; simpl.
-    destruct (dec_eq y x); subst; reflexivity.
+    destruct (string_dec y x); subst; reflexivity.
   Qed.
 
   Lemma substl_trunc_notin x' xs es :
     ~ In x' xs ->
-    substl_trunc (zip xs es) x' = @empty_open _ R.
+    substl_trunc (zip xs es) x' = @empty_open R.
   Proof.
     intro HnotIn. revert es. induction xs as [|x]; intros.
     + simpl. destruct es; reflexivity.
-    + destruct es as [|e]; [reflexivity|]. simpl. destruct (dec_eq x' x) as [|_].
+    + destruct es as [|e]; [reflexivity|]. simpl. destruct (string_dec x' x) as [|_].
       - subst. contradiction HnotIn. simpl. auto.
       - apply IHxs. auto with datatypes.
   Qed.
 
-  Lemma subst1_trunc_singleton_stack {B} (p : open B) (s : @stack A R) x y :
-    p[{y/V //! x}] s = p (stack_add x (s y) (stack_empty A)).
+  Lemma subst1_trunc_singleton_stack {B} (p : open B) (s : @stack R) x y :
+    p[{y/V //! x}] s = p (stack_add x (s y) (stack_empty)).
   Proof.
     unfold apply_subst, subst1_trunc, stack_subst; simpl.
     apply f_equal.
     apply functional_extensionality.
     intro x'.
-    destruct (dec_eq x' x); subst.
+    destruct (string_dec x' x); subst.
     * rewrite stack_lookup_add.
       reflexivity.
     * rewrite stack_lookup_add2; [| auto].
@@ -186,40 +185,39 @@ Hint Rewrite @substl_subst1 : open.
 Hint Rewrite @substl_trunc_notin using assumption : open.
 
 Section MoreLemmas.
-  Context {A : Type} {Heq : DecidableEq A}.
   Context {R : ValNull}.
 
   Open Scope open_scope.
 
   Lemma subst_singleton {B} : 
-    forall x e (P : @open A R B), P[{e//x}] = P // ((x, e)::nil).
+    forall x e (P : @open R B), P[{e//x}] = P // ((x, e)::nil).
   Proof.
     reflexivity.
   Qed.
 
   Lemma subst_open_expr_nil {B} :
-    forall (e : @open A R B), (e // nil) = e.
+    forall (e : @open R B), (e // nil) = e.
   Proof.
     reflexivity.
   Qed.
 
   Lemma subst_var_cons_eq : 
-    forall (x:A) es (e : expr), ((x/V) // ((x, e)::es)) = e.
+    forall (x:string) es (e : expr), ((x/V) // ((x, e)::es)) = e.
   Proof.
     intros x es e.
     apply functional_extensionality; intros s; simpl.
     unfold var_expr, apply_subst, stack_subst. simpl.
-    case (dec_eq x x); intuition congruence.
+    case (string_dec x x); intuition congruence.
   Qed.
 
-  Lemma subst_var_cons_ineq : forall (x:A) y es (e : expr)
+  Lemma subst_var_cons_ineq : forall (x:string) y es (e : expr)
     (Hneq: x <> y),
     ((x/V) // ((y, e)::es)) = ((x/V) // es).
   Proof.
     intros x y es e Hneq.
     apply functional_extensionality; intros s.
     unfold var_expr, apply_subst, stack_subst; simpl.
-    case (dec_eq x y); congruence.
+    case (string_dec x y); congruence.
   Qed.
 
   Lemma val_expr_substs : forall (v : val) es,
@@ -229,10 +227,10 @@ Section MoreLemmas.
   Qed.
 
 
-  Definition subst_substlist (es fs : @substlist A R) : substlist :=
+  Definition subst_substlist (es fs : @substlist R) : substlist :=
     map (fun x => (fst x, (snd x) // fs)) es.
 
-  Lemma subst_combine {B} (e : @open A R B) (es fs : substlist) :
+  Lemma subst_combine {B} (e : @open R B) (es fs : substlist) :
     (e // es // fs) = (e // ((subst_substlist es fs)++fs)).
   Proof.
     apply functional_extensionality; intros s.
@@ -241,7 +239,7 @@ Section MoreLemmas.
     induction es; simpl.
     + reflexivity.
     + destruct a; simpl.
-      destruct (dec_eq x a); simpl.
+      destruct (string_dec x s0); simpl.
       * reflexivity.
       * apply IHes.
   Qed.
@@ -252,31 +250,29 @@ Close Scope open_scope.
 End MoreLemmas.
 
 Section SubstFresh.
-
-  Context {A : Type} `{HEq: DecidableEq A}.
   Context {R : ValNull}.
 
-    Definition subst_fresh (vs: A -> val) (xs: list A) : subst :=
-      fun x' => if In_dec dec_eq x' xs then V_expr (vs x') else var_expr x'.
+    Definition subst_fresh (vs: string -> val) (xs: list string) : subst :=
+      fun x' => if In_dec string_dec x' xs then V_expr (vs x') else var_expr x'.
 
-   Fixpoint subst_fresh_l (vs: A -> val) (xs: list A) : list (@expr A R) :=
+   Fixpoint subst_fresh_l (vs: string -> val) (xs: list string) : list (@expr R) :=
       match xs with
       | nil => nil
       | x::xs' => V_expr (vs x) :: subst_fresh_l vs xs'
       end.
 
     (* TODO: switch the two alt. definitions. *)
-    Lemma subst_fresh_alt (vs: A -> val) (xs: list A) :
+    Lemma subst_fresh_alt (vs: string -> val) (xs: list string) :
       subst_fresh vs xs = substl (zip xs (subst_fresh_l vs xs)).
     Proof.
       induction xs as [|x]; [reflexivity|].
       apply functional_extensionality.
-      intro x'. simpl. destruct (dec_eq x' x).
+      intro x'. simpl. destruct (string_dec x' x).
       + subst x'. unfold subst_fresh. simpl.
-        destruct (dec_eq x x); congruence.
+        destruct (string_dec x x); congruence.
       + rewrite <- IHxs. unfold subst_fresh.
-        simpl. destruct (dec_eq x x'); [congruence|].
-        destruct (in_dec dec_eq x' xs); reflexivity.
+        simpl. destruct (string_dec x x'); [congruence|].
+        destruct (in_dec string_dec x' xs); reflexivity.
     Qed.
 
 End SubstFresh.
