Charge!/src/Logics/ILInsts.v
@@ -1,5 +1,5 @@
 Require Import RelationClasses Setoid Morphisms.
-Require Import ILogic ILEmbed ILQuantTac.
+Require Import ILogic ILEmbed.
 
 Set Implicit Arguments.
 Unset Strict Implicit.
@@ -41,9 +41,10 @@ Section ILogic_Pre.
     lexists  A P := mk (fun t => Exists a, P a t) _
   |}. 
   Next Obligation.
-    lforallR t'' Ht'. lforallL t''.
+    apply lforallR; intro t''. apply lforallR; intro Ht'.
+    apply lforallL with t''.
     assert (ord t t'') as Ht'' by (transitivity t'; assumption).
-    lforallL Ht''; reflexivity.
+    apply lforallL with Ht''; reflexivity. 
   Defined.
 
   Local Existing Instance ILPre_Ops.
@@ -56,10 +57,10 @@ Section ILogic_Pre.
       transitivity (Q t); [apply HPQ | apply HQR].
     - apply ltrueR.
     - apply lfalseL.
-    - lforallL x; apply H. 
-    - lforallR x; apply H. 
-    - lexistsL x; apply H. 
-    - lexistsR x; apply H. 
+    - apply lforallL with x; apply H. 
+    - apply lforallR; intro x; apply H. 
+    - apply lexistsL; intro x; apply H. 
+    - apply lexistsR with x; apply H. 
     - apply landL1; eapply H; assumption.
     - apply landL2; eapply H; assumption.
     - apply lorR1; eapply H; assumption.
@@ -69,7 +70,7 @@ Section ILogic_Pre.
     - apply landAdj.
       etransitivity; [apply H|]. apply lforallL with t.
       apply lforallL; reflexivity.
-    - lforallR t' Hord. apply limplAdj.
+    - apply lforallR; intro t'; apply lforallR; intro Hord. apply limplAdj.
       rewrite ->Hord; eapply H; assumption.
   Qed.
 
@@ -103,7 +104,7 @@ Section ILogic_Pre.
   Program Definition ILPreAtom {HPre : PreOrder ord} (t: T) :=
     mk (fun t' => Exists x : ord t t', ltrue) _.
   Next Obligation.
-    lexistsL H1.
+    apply lexistsL; intro H1.
     apply lexistsR; [transitivity t0; assumption | apply ltrueR].
   Qed.
 
@@ -156,8 +157,8 @@ Section Embed_ILogic_Pre.
     + split; intros t; simpl; apply embedlforall.
     + split; intros t; simpl; apply embedlexists.
     + split; intros t; simpl. 
-      * lforallL t. apply lforallL; [reflexivity | apply embedImpl].
-      * lforallR x H. apply embedImpl.
+      * apply lforallL with t; apply lforallL; [reflexivity | apply embedImpl].
+      * apply lforallR; intro x; apply lforallR; intro H. apply embedImpl.
   Qed.
         
   Program Instance EmbedILPreOp : EmbedOp (ILPreFrm ord A) (ILPreFrm ord B) := {
@@ -175,7 +176,8 @@ Section Embed_ILogic_Pre.
     + split; intros t; simpl; apply embedlexists.
     + split; intros t; simpl;
       do 2 setoid_rewrite <- embedlforall; 
-      lforallR t' H; lforallL t' H; apply embedImpl.
+      apply lforallR; intro t'; apply lforallR; intro H; 
+      apply lforallL with t'; apply lforallL with H; apply embedImpl.
   Qed.
         
 End Embed_ILogic_Pre.
