Charge!/src/Open/OpenILogic.v
@@ -1,14 +1,13 @@
-Require Import ILogic ILEmbed ILInsts ILQuantTac Rel.
-Require Import Open Stack.
+Require Import ILogic ILEmbed ILInsts Rel.
+Require Import Open Stack String.
 
 Local Existing Instance ILFun_Ops.
 Local Existing Instance ILFun_ILogic.
 
 Section VLogic.
-  Context {A : Type} {Heq : DecidableEq A}.
   Context {V : ValNull}.
 
-  Definition vlogic := @open A V Prop.
+  Definition vlogic := @open V Prop.
 
   Definition open_eq {T} (a b : open T) : vlogic :=
     fun s => a s = b s.
@@ -37,10 +36,10 @@ Section Existentialise.
   Local Existing Instance EmbedILFunOp.
   Local Existing Instance EmbedILFun.
 
-  Lemma existentialise_var (x : A) (P : open B) : 
+  Lemma existentialise_var (x : string) (P : open B) : 
   	P |-- @lexists (open B) _ _ (fun v : val => @lembedand vlogic (open B) _ _ (open_eq (x/V) `v) P).
   Proof.
-  	intro s; unfold liftn, lift, var_expr, open_eq; simpl. lexistsR (s x). 	
+  	intro s; unfold liftn, lift, var_expr, open_eq; simpl. apply lexistsR with (s x). 	
   	apply landR; [apply embedPropR|]; reflexivity.
   Qed.
 End Existentialise.
